\input{commands}
\title{\bf CSE 401: Numerical Analysis \\ HW 5}
\author{Bhavesh Shrimali \\ NetID: bshrima2}
\date{\today}
\titlespacing*{\title}{-2ex}{*-2ex}{-2ex}
\begin{document}
\maketitle \hrule \hrule \hrule
\section*{Solution 3: Equivalent First Order System}
The equivalent first order linear ODE systems, for the given higher order ODEs are as follows: 
\subsection*{(a) Van der Pol Equation:}
\begin{align*}
y'' = y'(1-y^2) - y
\end{align*}
The equivalent first order system can be given by making the following substitution 
\begin{align*}
{\bf y} = 
\begin{Bmatrix}
y_1 \\
y_2
\end{Bmatrix}
=
\begin{Bmatrix}
y \\
y'
\end{Bmatrix}
\end{align*}
Thus we have 
\begin{align*}
{\bf y}'
=
\begin{Bmatrix}
y'_1\\y'_2
\end{Bmatrix}
=
\begin{Bmatrix}
y_2\\y_2(1-y^2_1)-y_1
\end{Bmatrix}
\end{align*}
We can therefore rewrite the system in the following form 
\begin{align*}
\boxed{
{\bf y}' = {\bf f}(t,{\bf y})\ \ \ ; \ \ \ \ {\bf y}' = \begin{Bmatrix}
y'_1\\y'_2
\end{Bmatrix}
\ \ \ \ \ {\bf f}(t,{\bf y}) = \begin{Bmatrix}
y_2\\y_2(1-y^2_1)-y_1
\end{Bmatrix}
}
\end{align*} \hrule
\subsection*{(b) Blasius Equation}
Given ODE
\begin{align*}
y''' = -yy''
\end{align*}
We again make a similar substitution, as above, illustrated below 
\begin{align*}
{\bf y}
=
\begin{Bmatrix}
y_1\\y_2\\y_3
\end{Bmatrix}
=
\begin{Bmatrix}
y\\y'\\y''
\end{Bmatrix}
\end{align*}
Thus our equivalent first order ODE system is 
\begin{align*}
\boxed{
{\bf y}'
=
{\bf f}(t,{\bf y}) \ \ \ \ ; {\bf y}'
=
\begin{Bmatrix}
y'_1\\y'_2\\y'_3
\end{Bmatrix}
 \ \ \ \ \ \ {\bf f}(t,{\bf y}) = 
\begin{Bmatrix}
y_2\\y_3\\-y_1\cdot y_3
\end{Bmatrix}
}
\end{align*}
\subsection*{(c) Newton's Second Law-Two Body Problem}
Given ODE system
\begin{align*}
\begin{Bmatrix}
{y}''_1\\{y}''_2
\end{Bmatrix}
= - \frac{GM}{(y^2_1+y^2_2)^{3/2}}
\begin{Bmatrix}
y_1\\y_2
\end{Bmatrix}
\end{align*}
Let $$ k (y_1,y_2) = \frac{GM}{(y^2_1+y^2_2)^{3/2}}$$
Using this we make the substitution given below: 
\begin{align*}
{\bf y}
=
\begin{Bmatrix}
y_{11}\\y_{12}\\y_{21}\\y_{22}
\end{Bmatrix}
=
\begin{Bmatrix}
y_1\\y'_1\\y_2\\y'_2
\end{Bmatrix}
\implies 
{\bf y}' = 
\begin{Bmatrix}
y'_1\\y''_1\\y'_2\\y''_2
\end{Bmatrix}
=
\begin{Bmatrix}
y_{12}\\-ky_{11}\\y_{22}\\-ky_{21}
\end{Bmatrix}
\end{align*}
Thus our corresponding linear first order system is given by 
\begin{align*}
\boxed{
{\bf y}' = {\bf f}(t,{\bf y})\ \ \ ; \ \ \ \ \ {\bf y}' = \begin{Bmatrix}
y'_{11}\\y'_{12}\\y'_{21}\\y'_{22}
\end{Bmatrix} \ \ \ \ \ \ \ {\bf f}(t,{\bf y})
=
\begin{Bmatrix}
y_{12}\\-k(y_{11},y_{21})\cdot y_{11}\\y_{22}\\-k(y_{11},y_{21})\cdot y_{21}
\end{Bmatrix}
}
\end{align*}\hrule\hrule\hrule
\end{document}